CollapsingTowers/TwoLevelPCP/Shift.lean
@@ -1,6 +1,24 @@
 
 import CollapsingTowers.TwoLevelPCP.Syntax
 import CollapsingTowers.TwoLevelPCP.OpenClose
+
+@[simp]
+def shiftl_at (x : ℕ) (n : ℕ) : Expr -> Expr
+  | .bvar i => .bvar i
+  | .fvar y => if x <= y then .fvar (y + n) else .fvar y
+  | .lam₁ e => .lam₁ (shiftl_at x n e)
+  | .lift e => .lift (shiftl_at x n e)
+  | .app₁ f arg => .app₁ (shiftl_at x n f) (shiftl_at x n arg)
+  | .app₂ f arg => .app₂ (shiftl_at x n f) (shiftl_at x n arg)
+  | .lit₁ n => .lit₁ n
+  | .plus₁ l r => .plus₁ (shiftl_at x n l) (shiftl_at x n r)
+  | .plus₂ l r => .plus₂ (shiftl_at x n l) (shiftl_at x n r)
+  | .code e => .code (shiftl_at x n e)
+  | .reflect e => .reflect (shiftl_at x n e)
+  | .lam𝕔 e => .lam𝕔 (shiftl_at x n e)
+  | .lets b e => .lets (shiftl_at x n b) (shiftl_at x n e)
+  | .let𝕔 b e => .let𝕔 (shiftl_at x n b) (shiftl_at x n e)
+
 @[simp]
 def shiftr_at (x : ℕ) : Expr -> Expr
   | .bvar i => .bvar i
@@ -17,3 +35,194 @@ def shiftr_at (x : ℕ) : Expr -> Expr
   | .lam𝕔 e => .lam𝕔 (shiftr_at x e)
   | .lets b e => .lets (shiftr_at x b) (shiftr_at x e)
   | .let𝕔 b e => .let𝕔 (shiftr_at x b) (shiftr_at x e)
+
+theorem shiftl_opening :
+    ∀ x y e n i, x <= y -> shiftl_at x n (opening i (.fvar y) e) = opening i (.fvar (y + n)) (shiftl_at x n e) :=
+  by
+  intros x y e n i HLe
+  induction e generalizing i with
+  | bvar j =>
+    by_cases HEq : j = i
+    . rw [HEq]; simp; omega
+    . simp; rw [if_neg HEq]; rw [if_neg HEq]; rfl
+  | fvar z =>
+    by_cases HLe : x <= z
+    . simp; rw [if_pos HLe]; rfl
+    . simp; rw [if_neg HLe]; rfl
+  | app₁ _ _ IH₀ IH₁
+  | app₂ _ _ IH₀ IH₁
+  | plus₁ _ _ IH₀ IH₁
+  | plus₂ _ _ IH₀ IH₁
+  | lets _ _ IH₀ IH₁
+  | let𝕔 _ _ IH₀ IH₁ =>
+    simp; constructor; apply IH₀; apply IH₁
+  | lit₁ => simp
+  | lam₁ _ IH
+  | lift _ IH
+  | lam𝕔 _ IH
+  | code _ IH
+  | reflect _ IH =>
+    simp; apply IH
+
+theorem shiftl_open₀ : ∀ x y e n, x <= y -> shiftl_at x n (open₀ y e) = open₀ (y + n) (shiftl_at x n e) := by
+  intros _ _ _ _; apply shiftl_opening
+
+theorem shiftl_closed_at :
+    ∀ x y e n, closed_at e x -> closed_at (shiftl_at y n e) (x + n) :=
+  by
+  intros x y e n Hclose
+  induction e with
+  | bvar j => simp
+  | fvar z =>
+    by_cases HLe : y <= z
+    . simp; rw [if_pos HLe]; simp; apply Hclose
+    . simp; rw [if_neg HLe]; simp at *; omega
+  | app₁ _ _ IH₀ IH₁
+  | app₂ _ _ IH₀ IH₁
+  | plus₁ _ _ IH₀ IH₁
+  | plus₂ _ _ IH₀ IH₁
+  | lets _ _ IH₀ IH₁
+  | let𝕔 _ _ IH₀ IH₁ =>
+    simp; constructor
+    apply IH₀; apply Hclose.left
+    apply IH₁; apply Hclose.right
+  | lit₁ => simp
+  | lam₁ _ IH
+  | lift _ IH
+  | lam𝕔 _ IH
+  | code _ IH
+  | reflect _ IH =>
+    simp; apply IH; apply Hclose
+
+theorem shiftl_id :
+    ∀ x e n, closed_at e x -> shiftl_at x n e = e :=
+  by
+  intros x e n
+  induction e with
+  | bvar j => simp
+  | fvar y => simp; omega
+  | app₁ _ _ IH₀ IH₁
+  | app₂ _ _ IH₀ IH₁
+  | plus₁ _ _ IH₀ IH₁
+  | plus₂ _ _ IH₀ IH₁
+  | lets _ _ IH₀ IH₁
+  | let𝕔 _ _ IH₀ IH₁ =>
+    intro Hclose; simp; constructor
+    apply IH₀; apply Hclose.left
+    apply IH₁; apply Hclose.right
+  | lit₁ => simp
+  | lam₁ _ IH
+  | lift _ IH
+  | lam𝕔 _ IH
+  | code _ IH
+  | reflect _ IH =>
+    simp; apply IH
+
+theorem shiftr_opening_comm :
+    ∀ x y e i, x < y -> shiftr_at x (opening i (.fvar y) e) = opening i (.fvar (y - 1)) (shiftr_at x e) :=
+  by
+  intros x y e i HLe
+  induction e generalizing i with
+  | bvar j =>
+    by_cases HEq : j = i
+    . rw [HEq]; simp; omega
+    . simp; rw [if_neg HEq, if_neg HEq]; simp
+  | fvar z =>
+    by_cases HLe : x < z
+    . simp; rw [if_pos HLe]; rfl
+    . simp; rw [if_neg HLe]; rfl
+  | app₁ _ _ IH₀ IH₁
+  | app₂ _ _ IH₀ IH₁
+  | plus₁ _ _ IH₀ IH₁
+  | plus₂ _ _ IH₀ IH₁
+  | lets _ _ IH₀ IH₁
+  | let𝕔 _ _ IH₀ IH₁ =>
+    simp; constructor; apply IH₀; apply IH₁
+  | lit₁ => simp
+  | lam₁ _ IH
+  | lift _ IH
+  | lam𝕔 _ IH
+  | code _ IH
+  | reflect _ IH =>
+    simp; apply IH
+
+theorem shiftr_open₀_comm : ∀ x y e, x < y -> shiftr_at x (open₀ y e) = open₀ (y - 1) (shiftr_at x e) :=
+  by
+  intros _ _ _
+  apply shiftr_opening_comm
+
+theorem shiftr_closed_at : ∀ x y e, y < x -> closed_at e (x + 1) -> closed_at (shiftr_at y e) x :=
+  by
+  intros x y e Hxy Hclose
+  induction e with
+  | bvar j => simp
+  | fvar z =>
+    by_cases Hyz : y < z
+    . simp; rw [if_pos Hyz]; simp at *; omega
+    . simp; rw [if_neg Hyz]; simp at *; omega
+  | app₁ _ _ IH₀ IH₁
+  | app₂ _ _ IH₀ IH₁
+  | plus₁ _ _ IH₀ IH₁
+  | plus₂ _ _ IH₀ IH₁
+  | lets _ _ IH₀ IH₁
+  | let𝕔 _ _ IH₀ IH₁ =>
+    simp; constructor
+    apply IH₀; apply Hclose.left
+    apply IH₁; apply Hclose.right
+  | lit₁ => simp
+  | lam₁ _ IH
+  | lift _ IH
+  | lam𝕔 _ IH
+  | code _ IH
+  | reflect _ IH =>
+    simp; apply IH; apply Hclose
+
+theorem shiftr_closed_at_id : ∀ x e, closed_at e x -> closed_at (shiftr_at x e) x :=
+  by
+  intros x e Hclose
+  induction e with
+  | bvar j => simp
+  | fvar z =>
+    by_cases Hxz : x < z
+    . simp; rw [if_pos Hxz]; simp at *; omega
+    . simp; rw [if_neg Hxz]; simp at *; omega
+  | app₁ _ _ IH₀ IH₁
+  | app₂ _ _ IH₀ IH₁
+  | plus₁ _ _ IH₀ IH₁
+  | plus₂ _ _ IH₀ IH₁
+  | lets _ _ IH₀ IH₁
+  | let𝕔 _ _ IH₀ IH₁ =>
+    simp; constructor
+    apply IH₀; apply Hclose.left
+    apply IH₁; apply Hclose.right
+  | lit₁ => simp
+  | lam₁ _ IH
+  | lift _ IH
+  | lam𝕔 _ IH
+  | code _ IH
+  | reflect _ IH =>
+    simp; apply IH; apply Hclose
+
+theorem shiftr_id :
+    ∀ x e, closed_at e (x + 1) -> shiftr_at x e = e :=
+  by
+  intros x e
+  induction e with
+  | bvar j => simp
+  | fvar y => simp; omega
+  | app₁ _ _ IH₀ IH₁
+  | app₂ _ _ IH₀ IH₁
+  | plus₁ _ _ IH₀ IH₁
+  | plus₂ _ _ IH₀ IH₁
+  | lets _ _ IH₀ IH₁
+  | let𝕔 _ _ IH₀ IH₁ =>
+    intro Hclose; simp; constructor
+    apply IH₀; apply Hclose.left
+    apply IH₁; apply Hclose.right
+  | lit₁ => simp
+  | lam₁ _ IH
+  | lift _ IH
+  | lam𝕔 _ IH
+  | code _ IH
+  | reflect _ IH =>
+    simp; apply IH
