CollapsingTowers/TwoLevelPCP/Preservation.lean
@@ -1,4 +1,5 @@
 
+import Mathlib.Tactic
 import CollapsingTowers.TwoLevelPCP.Typing
 import CollapsingTowers.TwoLevelPCP.Shift
 @[simp]
@@ -12,44 +13,222 @@ theorem preservation_subst_strengthened :
       typing Φ .stat v τ𝕒 ∅ ->
       typing (Δ ++ Φ) .stat (shiftr_at Φ.length (subst Φ.length v e)) τ𝕓 φ :=
   by
-  generalize Eq𝕊 : Stage.stat = 𝕊
   intros Γ Δ Φ v e τ𝕒 τ𝕓 φ Hτe HEqΓ Hτv
   revert Δ
   apply
     @typing.rec
       (fun Γ 𝕊 e τ𝕓 φ (H : typing Γ 𝕊 e τ𝕓 φ) =>
-        ∀ (Δ : TEnv), Γ = Δ ++ (τ𝕒, 𝕊) :: Φ → typing (Δ ++ Φ) 𝕊 (shiftr_at Φ.length (subst Φ.length v e)) τ𝕓 φ)
+        ∀ (Δ : TEnv), Γ = Δ ++ (τ𝕒, .stat) :: Φ →
+          typing (Δ ++ Φ) 𝕊 (shiftr_at Φ.length (subst Φ.length v e)) τ𝕓 φ)
       (fun Γ e τ𝕓 φ (H : typing_reification Γ e τ𝕓 φ) =>
-        ∀ (Δ : TEnv),
-          Γ = Δ ++ (τ𝕒, 𝕊) :: Φ → typing_reification (Δ ++ Φ) (shiftr_at Φ.length (subst Φ.length v e)) τ𝕓 φ)
+        ∀ (Δ : TEnv), Γ = Δ ++ (τ𝕒, .stat) :: Φ →
+          typing_reification (Δ ++ Φ) (shiftr_at Φ.length (subst Φ.length v e)) τ𝕓 φ)
   case fvar =>
-    intros _ _ x _ Hbinds Δ HEqΓ
-    admit
+    intros _ 𝕊 x _ Hbinds Δ HEqΓ
+    rw [HEqΓ] at Hbinds; simp
+    cases Hx : compare Φ.length x with
+    | lt =>
+      rw [compare_lt_iff_lt] at Hx
+      rw [if_neg (Nat.ne_of_lt Hx)]
+      simp; rw [if_pos Hx]
+      constructor
+      have Hx : Φ.length <= x - 1 := by omega
+      rw [← Nat.add_sub_of_le Hx, Nat.add_comm]
+      apply binds_extendr
+      rw [← Nat.sub_add_eq, Nat.add_comm]
+      apply binds_shrinkr _ ((τ𝕒, .stat) :: Φ)
+      rw [List.length_cons, Nat.sub_add_cancel]
+      apply Hbinds; omega
+    | eq =>
+      rw [compare_eq_iff_eq] at Hx
+      rw [← Hx] at Hbinds; apply binds_shrink at Hbinds
+      simp at Hbinds; rw [← Hbinds.left, ← Hbinds.right]
+      rw [if_pos Hx]; rw [shiftr_id]
+      apply weakening; apply Hτv
+      apply closed_inc; apply typing_closed
+      apply Hτv; omega; simp
+    | gt =>
+      rw [compare_gt_iff_gt] at Hx
+      rw [if_neg (Nat.ne_of_gt Hx)]
+      simp; rw [if_neg (Nat.not_lt_of_gt Hx)]
+      constructor
+      apply binds_extend; apply binds_shrink
+      omega; rw [List.append_cons] at Hbinds; apply Hbinds
   case lam₁ =>
     intros _ _ _ _ _ _ _ HwellBinds Hclose IH Δ HEqΓ
-    admit
+    rw [HEqΓ] at IH; rw [HEqΓ] at Hclose
+    rw [subst_open₀_comm, shiftr_open₀_comm] at IH
+    apply typing.lam₁
+    simp; rw [← List.cons_append]
+    simp at IH; apply IH; rfl
+    apply HwellBinds
+    cases Δ with
+    | nil =>
+      apply shiftr_closed_at_id; apply subst_closed_at_dec
+      apply typing_closed; apply Hτv; apply Hclose
+    | cons =>
+      simp at *
+      apply shiftr_closed_at; omega
+      apply subst_closed_at; apply closed_inc
+      apply typing_closed; apply Hτv; omega; apply Hclose
+    simp; omega
+    simp; omega
+    apply typing_regular; apply Hτv
+  case lift_lam =>
+    intros _ _ _ _ _ _ _ IH Δ HEqΓ
+    apply typing.lift_lam
+    apply IH; apply HEqΓ
+  case lam𝕔 =>
+    intros _ _ _ _ _ _ HwellBinds Hclose IH Δ HEqΓ
+    rw [HEqΓ] at IH; rw [HEqΓ] at Hclose
+    rw [subst_open₀_comm, shiftr_open₀_comm] at IH
+    apply typing.lam𝕔
+    simp; rw [← List.cons_append]
+    simp at IH; apply IH; rfl
+    apply HwellBinds
+    cases Δ with
+    | nil =>
+      apply shiftr_closed_at_id; apply subst_closed_at_dec
+      apply typing_closed; apply Hτv; apply Hclose
+    | cons =>
+      simp at *
+      apply shiftr_closed_at; omega
+      apply subst_closed_at; apply closed_inc
+      apply typing_closed; apply Hτv; omega; apply Hclose
+    simp; omega
+    simp; omega
+    apply typing_regular; apply Hτv
   case app₁ =>
     intros _ _ _ _ _ _ _ _ _ _ _ IHf IHarg Δ HEqΓ
-    constructor
+    apply typing.app₁
     apply IHf; apply HEqΓ
     apply IHarg; apply HEqΓ
   case app₂ =>
     intros _ _ _ _ _ _ _ _ _ IHf IHarg Δ HEqΓ
-    constructor
+    apply typing.app₂
     apply IHf; apply HEqΓ
     apply IHarg; apply HEqΓ
-  case lam𝕔 =>
-    intros _ _ _ _ _ _ HwellBinds Hclose IH Δ HEqΓ
-    admit
+  case plus₁ =>
+    intros _ _ _ _ _ _ _ _ IHl IHr Δ HEqΓ
+    apply typing.plus₁
+    apply IHl; apply HEqΓ
+    apply IHr; apply HEqΓ
+  case plus₂ =>
+    intros _ _ _ _ _ _ _ IHl IHr Δ HEqΓ
+    apply typing.plus₂
+    apply IHl; apply HEqΓ
+    apply IHr; apply HEqΓ
+  case lit₁ => intros; apply typing.lit₁
+  case lift_lit =>
+    intros _ _ _ _ IH Δ HEqΓ
+    apply typing.lift_lit
+    apply IH; apply HEqΓ
+  case code₁ =>
+    intros _ x _ Hbinds Δ HEqΓ
+    rw [HEqΓ] at Hbinds; simp
+    cases Hx : compare Φ.length x with
+    | lt =>
+      rw [compare_lt_iff_lt] at Hx
+      rw [if_neg (Nat.ne_of_lt Hx)]
+      simp; rw [if_pos Hx]
+      apply typing.code₁
+      have Hx : Φ.length <= x - 1 := by omega
+      rw [← Nat.add_sub_of_le Hx, Nat.add_comm]
+      apply binds_extendr
+      rw [← Nat.sub_add_eq, Nat.add_comm]
+      apply binds_shrinkr _ ((τ𝕒, .stat) :: Φ)
+      rw [List.length_cons, Nat.sub_add_cancel]
+      apply Hbinds; omega
+    | eq =>
+      rw [compare_eq_iff_eq] at Hx
+      rw [← Hx] at Hbinds; apply binds_shrink at Hbinds
+      simp at Hbinds; simp
+    | gt =>
+      rw [compare_gt_iff_gt] at Hx
+      rw [if_neg (Nat.ne_of_gt Hx)]
+      simp; rw [if_neg (Nat.not_lt_of_gt Hx)]
+      apply typing.code₁
+      apply binds_extend; apply binds_shrink
+      omega; rw [List.append_cons] at Hbinds; apply Hbinds
+  case code₂ =>
+    intros _ _ _ _ IH Δ HEqΓ
+    apply typing.code₂
+    apply IH; apply HEqΓ
+  case reflect =>
+    intros _ _ _ _ IH Δ HEqΓ
+    apply typing.reflect
+    apply IH; apply HEqΓ
+  case lets =>
+    intros _ _ _ _ _ _ _ _ _ _ HwellBinds Hclose IHb IHe Δ HEqΓ
+    rw [HEqΓ] at IHb; rw [HEqΓ] at IHe; rw [HEqΓ] at Hclose
+    rw [subst_open₀_comm, shiftr_open₀_comm] at IHe
+    simp at IHb; simp at IHe
+    apply typing.lets
+    apply IHb
+    simp; rw [← List.cons_append]; apply IHe; rfl
+    apply HwellBinds
+    cases Δ with
+    | nil =>
+      simp at *; apply shiftr_closed_at_id
+      apply subst_closed_at_dec
+      apply typing_closed; apply Hτv
+      apply Hclose
+    | cons =>
+      simp at *; apply shiftr_closed_at; omega
+      apply subst_closed_at
+      apply closed_inc; apply typing_closed; apply Hτv; omega
+      apply Hclose
+    simp; omega
+    simp; omega
+    apply typing_regular; apply Hτv
+  case let𝕔 =>
+    intros _ _ _ _ _ _ _ _ HwellBinds Hclose IHb IHe Δ HEqΓ
+    rw [HEqΓ] at IHb; rw [HEqΓ] at IHe; rw [HEqΓ] at Hclose
+    rw [subst_open₀_comm, shiftr_open₀_comm] at IHe
+    simp at IHb; simp at IHe
+    apply typing.let𝕔
+    apply IHb
+    simp; rw [← List.cons_append]; apply IHe; rfl
+    apply HwellBinds
+    cases Δ with
+    | nil =>
+      simp at *; apply shiftr_closed_at_id
+      apply subst_closed_at_dec
+      apply typing_closed; apply Hτv
+      apply Hclose
+    | cons =>
+      simp at *; apply shiftr_closed_at; omega
+      apply subst_closed_at
+      apply closed_inc; apply typing_closed; apply Hτv; omega
+      apply Hclose
+    simp; omega
+    simp; omega
+    apply typing_regular; apply Hτv
   case pure =>
     intros _ _ _ _ IH Δ HEqΓ
     apply typing_reification.pure
-    apply IH; rw [Eq𝕊]; apply HEqΓ
+    apply IH; apply HEqΓ
   case reify =>
     intros _ _ _ _ IH Δ HEqΓ
     apply typing_reification.reify
-    apply IH; rw [Eq𝕊]; apply HEqΓ
-  all_goals admit
+    apply IH; apply HEqΓ
+  apply Hτe
+
+theorem preservation_subst :
+    ∀ Γ v e τ𝕒 τ𝕓 φ,
+      typing Γ .stat v τ𝕒 ∅ ->
+      typing ((τ𝕒, .stat) :: Γ) .stat e τ𝕓 φ ->
+      typing Γ .stat (subst Γ.length v e) τ𝕓 φ :=
+  by
+  intros Γ v e τ𝕒 τ𝕓 φ Hτv Hτe
+  have H := preservation_subst_strengthened ((τ𝕒, .stat) :: Γ) [] Γ v e τ𝕒 τ𝕓 φ
+  simp at H
+  have H := H Hτe Hτv
+  rw [shiftr_id] at H
+  apply H
+  apply subst_closed_at
+  apply closed_inc; apply typing_closed; apply Hτv; omega
+  rw [← List.length_cons]; apply typing_closed; apply Hτe
 
 theorem preservation_head𝕄 :
     ∀ Γ e₀ e₁ τ φ,
@@ -61,7 +240,16 @@ theorem preservation_head𝕄 :
   by
   intros Γ e₀ e₁ τ φ HdynΓ Hhead Hlc Hτ
   cases Hhead
-  case lets Hvalue => admit
+  case lets Hvalue =>
+    cases Hτ
+    case lets e v τ φ _ _ Hτv Hclose Hτe =>
+    have Hpure : φ = ∅ := by
+      apply typing_pure
+      apply Hτv; apply Hvalue
+    rw [Hpure] at Hτv; rw [Hpure, open_subst, union_pure_left]
+    rw [← subst_intro]
+    apply preservation_subst
+    apply Hτv; apply Hτe; apply Hclose
   all_goals admit
 
 theorem preservation_strengthened :
