CollapsingTowers/TwoLevelPCP/Typing.lean
@@ -77,3 +77,15 @@ mutual
     | pure : ∀ Γ e τ, typing Γ .stat e τ ∅ -> typing_reification Γ e τ ∅
     | reify : ∀ Γ e τ, typing Γ .stat e (.fragment τ) .reify -> typing_reification Γ e (.rep τ) .reify
 end
+
+theorem typing_regular : ∀ Γ 𝕊 e τ φ, typing Γ 𝕊 e τ φ -> lc e :=
+  by admit
+
+theorem typing_closed : ∀ Γ 𝕊 e τ φ, typing Γ 𝕊 e τ φ -> closed_at e Γ.length :=
+  by admit
+
+theorem typing_pure : ∀ Γ v τ φ, typing Γ .stat v τ φ -> value v -> φ = ∅ :=
+  by admit
+
+theorem weakening : ∀ Γ Δ 𝕊 e τ φ, typing Γ 𝕊 e τ φ -> typing (Δ ++ Γ) 𝕊 e τ φ :=
+  by admit
